\begin{equation}\label{q2_1}
\sqrt{dx^2 + dy^2 + dz^2}
\end{equation}
\begin{equation}\label{q2_2}
\begin{aligned}
x &= R \sin v \cos u\\
dx &= R \cos v \cos u du - R \sin v \sin u du\\
y &= R \sin v \sin u\\
dy &= R \cos v \sin u dv + R \sin v \cos u du\\
z = R \cos v\\
dz = -R \sin v dv\\
\end{aligned}
\end{equation}
Insert \ref{q2_2} into \ref{q2_1}
\begin{equation}
\begin{aligned}
\sqrt{(R \cos v \cos u du - R \sin v \sin u du)^2 + (R \cos v \sin u dv + R \sin v \cos u du)^2 + (-R \sin v dv)^2}
\end{aligned}
\end{equation}
First, let simplify the term inside the square root.
\begin{equation}
\begin{aligned}
R \cos v \cos u du - R \sin v \sin u du)^2 + (R \cos v \sin u dv + R \sin v \cos u du)^2 + (-R \sin v dv)^2\\
\;= R^2 \cos^2 v \cos^2 u dv^2 - 2 R \cos v \cos u \sin v \sin u dv du + R^2 \sin^2 v \sin^2 u du^2 \\
\;\;+ R^2 \cos^2 v \sin^2 u dv^2 + 2 R \cos v \cos u \sin v \sin u dv du + R^2 \sin^2 v \cos^2 u du^2 \\
\;\;+ R^2 \sin^2 v dv^2\\
\;= R^2 \cos^2 v \cos^2 u dv^2 + R^2 \sin^2 v \sin^2 u du^2 + R^2 \cos^2 v \sin^2 u dv^2 + R^2 \sin^2 v \cos^2 u du^2 + R^2 \sin^2 v dv^2\\
\;= R^2 (\sin^2 v du^2 (\sin^2 u + \cos^2 u) + \cos^2 v dv^2(\cos^2 u + \sin^2 u) + \sin^2 v dv^2)\\
\;= R^2 (\sin^2 v du^2 + \cos^2 v dv^2 + \sin^2 v dv^2)\\
\;= R^2 (\sin^2 v du^2 + dv^2(\cos^2 v + \sin^2 v))\\
\;= R^2 (\sin^2 v du^2 + dv^2\\
\end{aligned}
\end{equation}
Plug the equation back, we will get
\begin{equation}
\begin{aligned}
\sqrt{R^2 (\sin^2 v du^2 + dv^2} &= \sqrt{R^2} \sqrt{\sin^2 v du^2 + dv^2}\\
&= R \sqrt{\sin^2 v du^2 + dv^2}\\
&= R \sqrt{\sin^2 v du^2 + dv^2 \frac{du^2}{du^2}}\\
\end{aligned}
\end{equation}
Let's define $v' = \frac{dv}{du}$
\begin{equation}
\begin{aligned}
R \sqrt{\sin^2 v du^2 + dv^2 \frac{du^2}{du^2}} &= R \sqrt{\sin^2 v du^2 + dv^2 \frac{du^2}{du^2}}\\
&= R \sqrt{\sin^2 v du^2 + v'^2 du^2}\\
&= R \sqrt{du^2(\sin^2 v + v'^2)}\\
&= R \sqrt{\sin^2 v + v'^2} du\\
\end{aligned}
\end{equation}
Our arc length function will be now
\begin{equation}
L = R \int \sqrt{\sin^2 v + v'^2} du\\
\end{equation}
Our $F$ function will be
\begin{equation}
 \sqrt{\sin^2 v + v'^2}\\
\end{equation}
It's partial derivate to relative to $v'$ is
\begin{equation}
\begin{aligned}
 F_{v'} &= \frac{\partial}{\partial v'} \sqrt{\sin^2 v + v'^2}\\
 &= \frac{1}{2} (\sin^2 v + v'^2)^{-\frac{1}{2}} 2v'\\
 &= \frac{v'}{\sin^2 v + v'^2}
\end{aligned}
\end{equation}
Because $F$ does, not relies on $u$, the following is true:
\begin{equation}
v'F_{v'} - F = C
\end{equation}